CBPV/Soundness.lean
@@ -28,6 +28,12 @@ notation:40 Γ:41 "⊨" m:41 "∶" B:41 => semCom Γ m B
   Fundamental soundness theorem
 ------------------------------*-/
 
+theorem SNup {Γ σ A B P} {m : Com}
+  (hσ : Γ ⊨ σ) (hA : ⟦ A ⟧ᵛ ↘ P) (h : Γ ∷ A ⊨ m ∶ B) : SNCom (m⦃⇑ σ⦄) := by
+  let ⟨Q, hB, qm⟩ := h (var 0 +: σ) (semCtxtCons hA (hA.sneVal .var) hσ)
+  rw [substComVar] at qm
+  exact (hB.snCom qm).antirenaming
+
 theorem soundness {Γ} :
   (∀ (v : Val) A, Γ ⊢ v ∶ A → Γ ⊨ v ∶ A) ∧
   (∀ (m : Com) B, Γ ⊢ m ∶ B → Γ ⊨ m ∶ B) := by
@@ -37,7 +43,15 @@ theorem soundness {Γ} :
   case var A mem =>
     let ⟨P, hA⟩ := A.interp
     exact ⟨P, hA, hσ mem hA⟩
-  case unit => exact ⟨_, .Unit, Or.inr .refl⟩
+  case unit => exact ⟨_, .Unit, .inr .refl⟩
+  case inl A₂ _ ih =>
+    let ⟨_, hA₂⟩ := A₂.interp
+    let ⟨_, hA₁, pv⟩ := ih σ hσ
+    refine ⟨_, .Sum hA₁ hA₂, .inr (.inl ⟨_, .refl, pv⟩)⟩
+  case inr A₁ _ _ ih =>
+    let ⟨_, hA₁⟩ := A₁.interp
+    let ⟨_, hA₂, pv⟩ := ih σ hσ
+    refine ⟨_, .Sum hA₁ hA₂, .inr (.inr ⟨_, .refl, pv⟩)⟩
   case thunk ih =>
     let ⟨_, hB, pm⟩ := ih σ hσ
     exact ⟨_, .U hB, hB.closure (.once .thunk) pm⟩
@@ -66,14 +80,13 @@ theorem soundness {Γ} :
   case ret ih =>
     let ⟨_, hA, pv⟩ := ih σ hσ
     exact ⟨_, .F hA, Or.inr ⟨_, .refl, pv⟩⟩
-  case letin m n _ _ _ _ ihm ihn =>
+  case letin m n _ B _ _ ihm ihn =>
     let ⟨_, hFA, pm⟩ := ihm σ hσ
     cases hFA with | F hA =>
     match pm with
     | .inl ⟨_, r, sne⟩ =>
-      let ⟨P, hB, pn⟩ := ihn (var 0 +: σ) (semCtxtCons hA (hA.sneVal .var) hσ)
-      rw [substComVar] at pn
-      let plet := hB.sneCom (.letin sne (hB.snCom pn).antirenaming)
+      let ⟨P, hB⟩ := B.interp
+      let plet := hB.sneCom (.letin sne (SNup hσ hA ihn))
       exact ⟨P, hB, hB.closure (.letin r) plet⟩
     | .inr ⟨v, r, pv⟩ =>
       let ⟨_, hB, pn⟩ := ihn (v +: σ) (semCtxtCons hA pv hσ)
@@ -85,6 +98,35 @@ theorem soundness {Γ} :
           _ ⤳⋆ n⦃⇑ σ⦄⦃v⦄               := .once (.ret (hA.snVal pv))
           _ ⤳⋆ n⦃v +: σ⦄               := by rw [← substUnion]
       exact ⟨_, hB, hB.closure r' pn⟩
+  case case v m n _ _ B _ _ _ ihv ihm ihn =>
+    let ⟨_, hSum, pv⟩ := ihv σ hσ
+    cases hSum with | Sum hA₁ hA₂ =>
+      let snm := SNup hσ hA₁ ihm
+      let snn := SNup hσ hA₂ ihn
+      match pv with
+      | .inl sne =>
+        let ⟨P, hB⟩ := B.interp
+        exact ⟨P, hB, hB.sneCom (.case sne snm snn)⟩
+      | .inr (.inl ⟨w, r, pv⟩) =>
+        let ⟨R, hB, rm⟩ := ihm (w +: σ) (semCtxtCons hA₁ pv hσ)
+        let r' : (case v m n)⦃σ⦄ ⤳⋆ m⦃w +: σ⦄ := by
+          calc
+            (case v m n)⦃σ⦄
+            _ ⤳⋆ case (v⦃σ⦄) (m⦃⇑ σ⦄) (n⦃⇑ σ⦄) := .refl
+            _ ⤳⋆ case (inl w) (m⦃⇑ σ⦄) (n⦃⇑ σ⦄) := .case r
+            _ ⤳⋆ m⦃⇑ σ⦄⦃w⦄                      := .once (.inl snn)
+            _ ⤳⋆ m⦃w +: σ⦄                      := by rw [← substUnion]
+        exact ⟨R, hB, hB.closure r' rm⟩
+      | .inr (.inr ⟨w, r, qv⟩) =>
+        let ⟨R, hB, rm⟩ := ihn (w +: σ) (semCtxtCons hA₂ qv hσ)
+        let r' : (case v m n)⦃σ⦄ ⤳⋆ n⦃w +: σ⦄ := by
+          calc
+            (case v m n)⦃σ⦄
+            _ ⤳⋆ case (v⦃σ⦄) (m⦃⇑ σ⦄) (n⦃⇑ σ⦄) := .refl
+            _ ⤳⋆ case (inr w) (m⦃⇑ σ⦄) (n⦃⇑ σ⦄) := .case r
+            _ ⤳⋆ n⦃⇑ σ⦄⦃w⦄                      := .once (.inr snm)
+            _ ⤳⋆ n⦃w +: σ⦄                      := by rw [← substUnion]
+        exact ⟨R, hB, hB.closure r' rm⟩
 
 theorem normalization {Γ} :
   (∀ {v : Val} {A}, Γ ⊢ v ∶ A → SNVal v) ∧
